Switched from IMP to untyped lambda calculus. IMP doesn't work! But also translation in lambda calculus is simpler which should lead to easier proofs as well.

Bisimulation.v
@@ -1,28 +1,23 @@
+Require Import Strings.String.
 Require Import List.
-Require Import IMP.
+Require Import Lambda.
 Require Import TSO.
 Require Import SC.
 Require Import Util.
 Require Import Translation.
 
 
-Inductive related : (term * bool) -> (term * bool) -> Prop :=
-  | related_reflexive : forall e thread, related (e, thread) (e, thread)
-  | related_base1 : forall e thread, related (e, thread) (seq yunit (seq yunit e), thread)
-  | related_base2 : forall e thread, related (e, thread) (seq yunit e, thread)
-  | related_plus1 : forall e1 e1' thread n,
-                    related (e1, thread) (e1', thread) ->
-                    related (plus (num n) e1, thread) (plus (num n) e1', thread)
-  | related_plus2 : forall e1 e1' e2 thread,
-                    (forall n, e1 <> num n) ->
-                    related (e1, thread) (e1', thread) ->
-                    related (plus e1 e2, thread) (plus e1' e2, thread).
+(* Inductive related : (term * bool) -> (term * bool) -> Prop :=
+  | related_num : forall n thread base buf_size, related (num n, thread) (app (lam "x" (seq (nd_flush thread base buf_size) (var "x"))) (num n), thread)
+  | related_plus1 : forall e1 e1' n thread,
+                   related (e1, thread) (e1', thread) ->
+                   related (plus (num n) e1, thread) (plus (num n) e1', thread)
+  | related_plus2 : forall e1 e1' e2 thread ,
+                   (forall n, e1 <> num n) ->
+                   related (e1, thread) (e1', thread) ->
+                   related (plus e1 e2, thread) (plus e1' e2, thread).*)
 
-Fact step_related : forall e e' re event thread,
-                    step e event e' -> related (e, thread) (re, thread) ->
-                    (exists re', steps re re' /\ related (re, thread) (re', thread)).
-  Proof. 
-                               
+Definition related  (s t : term * bool) := (snd s = snd t) /\ (exists buf_size base, fst t = translate (fst s) (snd s) base buf_size).
 
 Definition related_terms (TSO_program : TSO.program) (SC_program : SC.program) (base : nat) : Prop :=
   let TSO1 := snd (fst TSO_program) in
@@ -90,103 +85,15 @@ Definition related_program (p : TSO_machine) (q : SC_machine) (f : nat -> nat) (
   let TSO_init := snd (fst (fst TSO_program)) in
   let SC_init := fst (fst (fst SC_program)) in
   let buf_size := fst (fst (fst TSO_program)) in
-  (TSO_init <> nil -> SC_init = translate_vars TSO_init buf_size) /\
+  (TSO_init <> nil -> SC_init = translate_arrays TSO_init buf_size) /\
   related_terms TSO_program SC_program B /\
   related_memory TSO_memory SC_memory B f.
 
 Theorem forward_bisimulation : forall p p' q f B,
   TSO.pstep p p' -> related_program p q f B -> (exists q', related_program p' q' f B /\ psteps q q').
 Proof. intros. inversion H; subst.
-  + destruct q. destruct p. repeat (destruct p). destruct m. destruct mem. destruct mem'. repeat (destruct p0). repeat (destruct p). destruct H0. simpl in *. destruct H4. destruct H4. destruct H6. simpl in *. subst. assert (l = translate_vars (xs ++ (size, init) :: nil) buffer). apply H0. intros C. symmetry in C. contradiction app_cons_not_nil with (x:=xs) (a:=(size, init)) (y:=nil). subst. remember (translate_vars xs buffer, t1, t0, while tru (SPECIAL (length xs) [num 0]::= ZERO)) as answer_p. unfold related_memory in H5. simpl in *. destruct H5. destruct H7. destruct H7. remember (update_mapping (length xs) x size m, allocate x (x + size - 1) init g) as answer_m. refine (ex_intro _ (answer_p, answer_m) _); subst. admit.
-  + destruct H0. simpl in *. destruct H3. destruct H3. destruct q. destruct p. destruct p. destruct p. simpl in *. clear H0. destruct H5. subst. generalize dependent t1. induction H1; subst; intros; inversion H3; subst.
-    ++ admit.
-    ++ admit.
-    ++ admit.
-    ++ admit.
-    ++ admit.
-    ++ admit.
-    ++ admit.
-    ++ admit.
-    ++ admit.
-    ++ admit.
-    ++ admit.
-    ++ admit.
-    ++ admit.
-    ++ admit.
-    ++ admit.
-    ++ admit.
-    ++ admit.
-    ++ admit.
-    ++ admit.
-    ++ admit.
-    ++ admit.
-    ++ admit.
-    ++ admit.
-    ++ admit.
-    ++ admit.
-    ++ admit.
-    ++ admit.
-    ++ admit.
-    ++ admit.
-    ++ admit.
-    ++ admit.
-    ++ admit.
-    ++ admit.
-    ++ admit.
-    ++ admit.
-    ++ admit.
-    ++ admit.
-    ++ admit.
-    ++ admit.
-    ++ admit.
-    ++ admit.
-    ++ admit.
-    ++ admit.
-    ++ admit.
-    ++ admit.
-    ++ admit.
-    ++ admit.
-    ++ admit.
-    ++ admit.
-    ++ admit.
-    ++ admit.
-    ++ admit.
-    ++ admit.
-    ++ admit.
-    ++ admit.
-    ++ admit.
-    ++ admit.
-    ++ admit.
-    ++ admit.
-    ++ admit.
-    ++ admit.
-    ++ admit.
-    ++ admit.
-    ++ admit.
-    ++ admit.
-    ++ admit.
-    ++ admit.
-    ++ admit.
-    ++ admit.
-    ++ admit.
-    ++ admit.
-    ++ admit.
-    ++ admit.
-    ++ admit.
-    ++ admit.
-    ++ admit.
-    ++ admit.
-    ++ admit.
-    ++ admit.
-    ++ admit.
-    ++ admit.
-    ++ admit.
-    ++ admit.
-    ++ admit.
-    ++ admit.
-    ++ admit.
-    ++ admit.
-    ++ admit.
+  + destruct q. destruct p. repeat (destruct p). destruct m. destruct mem. destruct mem'. repeat (destruct p0). repeat (destruct p). destruct H0. simpl in *. destruct H4. destruct H4. destruct H6. simpl in *. subst. assert (l = translate_arrays (xs ++ (size, init) :: nil) buffer). apply H0. intros C. symmetry in C. contradiction app_cons_not_nil with (x:=xs) (a:=(size, init)) (y:=nil). subst. remember (translate_arrays xs buffer, t1, t0, while tru (SPECIAL (length xs) [num 0]::= ZERO)) as answer_p. unfold related_memory in H5. simpl in *. destruct H5. destruct H7. destruct H7. remember (update_mapping (length xs) x size m, allocate x (x + size - 1) init g) as answer_m. refine (ex_intro _ (answer_p, answer_m) _); subst. admit.
+  + destruct H0. simpl in *. destruct H3. destruct H3. destruct q. destruct p. destruct p. destruct p. simpl in *. clear H0. destruct H5. subst. generalize dependent s1'. induction s1; intros;  inversion H1; subst; intros.
     ++ admit.
     ++ admit.
     ++ admit.
